Lambda/Syntax.v
@@ -1,18 +1,13 @@
-
-Axiom ff : False.
-Notation "???" := (False_rect _ ff).
-
 Require Import Metalib.Metatheory.
 
-Require Import Stlc.Definitions.
-Require Import LJm.Definitions.
+Require Import ELambda.Definitions.
+Require Import LambdaJm.Syntax.
 
-Module S := Stlc.Definitions.
-Module L := LJm.Definitions.
+Module S := ELambda.Definitions.
+Module L := LambdaJm.Syntax.
 
-Import L.LJmNotations.
-Import S.StlcNotations.
-
+Import S.ELambdaNotations.
+Import L.LambdaJmNotations.
 
 Inductive is_lambda : term -> Prop :=
 | il_var_b (n:nat) : is_lambda (var_b n)
@@ -44,6 +39,13 @@ Lemma il_app_inv6 t1 t2 t3 t4 : ~ is_lambda (app t1 (args t2 anil (cabs (app t3 
 Lemma il_app_inv7 t1 t2 t3 l c : ~ is_lambda (app t1 (args t2 (t3 ::: l) c)).
   intro H; inversion H; auto. Qed.
 
+(* the big assumption *)
+
+Lemma is_lambda_proofs_unique t :
+  forall (H1 : is_lambda t) (H2 : is_lambda t), H1 = H2.
+Admitted.
+
+
 (* Lemmas on substitution *)
 
 Lemma subst_preserves_il u x t :
@@ -66,18 +68,6 @@ Proof.
   - destruct s; auto.
   - auto.
 Qed.
-
-Lemma beta_preserves_il t1 t2 : is_lambda t1 -> betaT t1 t2 -> is_lambda t2.
-  intros.
-  induction H0.
-  - induction H0. inversion H. cbn.
-    inversion H5. apply open_preserves_il; trivial.
-  - induction H0. inversion H.
-Qed.
-
-(*******************
- * relationship with the external STLC 
- *******************)
 
 (* E ----> T *)
 
@@ -183,56 +173,6 @@ Proof.
  intros. unfold open. unfold openT. apply commut_opens_rec.
 Qed.
 
-(********
- * Preservation of typing
- ********)
-
-(* WIP: MP *)
-
-Lemma typing_implies_uniq G e A : typing G e A -> uniq G.
-  induction 1; trivial.
-Admitted.
-
-Theorem typing_preserved1 G e A : uniq G -> typing G e A -> typingT G (exp_to_terms e) A.
-  intros.
-  induction H0; simpl; auto.
-  - apply typingT_Right with (L:=L `union` dom G); intros.
-    simpl.
-    change (typingT ((x, T1) :: G) (openT (exp_to_terms e) (exp_to_terms (S.var_f x))) T2).
-    rewrite <- commut_opens.
-    apply H1; auto. 
-  - apply typingT_Cut with (A:=T1) (B:=T2).
-    + exact (IHtyping1 H).
-    + apply typingA_Leftm with (C:=T2).
-      * exact (IHtyping2 H).
-      * apply typingL_Ax. trivial.
-      * apply typingC_Select with (L:=dom G). intros.
-        apply typingT_Axiom.
-        -- auto.
-        -- auto.
-Qed.
-
-Theorem typing_preserved2 G t A : typingT G t A -> forall H : is_lambda t, typing G (term_to_exp2 t H) A.
-  intros.
-  admit.
-Admitted.
-
-
-(********
- * Simulation of Stlc beta reduction by LJm beta1 reduction --only one step so far
- ********)
-
-(* Definition of beta rule adapted from Stlc --in Stlc it already comes together with cbn closure *)
-
-Inductive beta : exp -> exp -> Prop :=
- | beta_base : forall (e1 e2:exp),
-     lc_exp (S.abs e1) ->
-     lc_exp e2 ->
-     beta (S.app  (S.abs e1) e2)  (open e1 e2).
-
-Hint Constructors beta.
-
-(*The lemmata that follow lead to the thm on the simulation of a beta step at STLC by a beta1 step in lJm*)
 
 Lemma lcT_from_lc_exp : forall e, lc_exp e -> lcT (exp_to_terms e).
 Proof.
@@ -244,34 +184,7 @@ Proof.
     + constructor; auto. constructor. intro. cbn. auto.
 Qed.
 
-Lemma bv_zero : forall n, lcT (abs (var_b n)) -> n=0.
-Proof.
-  intros. inversion H. pick fresh x.  specialize (H1 x). cbn in H1. destruct (lt_eq_lt_dec n 0).
-  - destruct s.
-    + inversion H1.
-    + trivial.
-  - inversion H1.
-Qed.
 
-
-(* Simulation of the beta rule ---without compatible closure --by beta1 of LJm *)
-
-Lemma sim_by_beta_term : forall e1 e2,
-    beta e1 e2 -> beta1T (exp_to_terms e1) (exp_to_terms e2).
-Proof.
-   intros. inversion H. simpl.  subst. rewrite  commut_opens. constructor.
-   - constructor. intro. inversion H0.
-     change ( lcT (openT (exp_to_terms e0) (exp_to_terms (S.var_f x)))).
-     rewrite <- commut_opens. specialize H3 with x. apply lcT_from_lc_exp. trivial.
-   - apply lcT_from_lc_exp. trivial.
-   - constructor. intro. cbn.  trivial.
-Qed.
-
-Lemma is_lambda_proofs_unique t :
-  forall (H1 : is_lambda t) (H2 : is_lambda t), H1 = H2.
-  Check is_lambda_ind.
-Admitted.
-  
 Lemma term_to_exp_commutes_open t u (H1:is_lambda t) (H2:is_lambda u) :
   forall k H, term_to_exp (open_term_wrt_term_rec k t u) H =
          open_exp_wrt_exp_rec k (term_to_exp t H1) (term_to_exp u H2).
@@ -296,6 +209,29 @@ Proof.
       rewrite <- (is_lambda_proofs_unique _ H1 H5). trivial.
 Qed.
 
+
+Lemma term_to_exp_preserves_lc: forall t,
+    forall H, lcT t -> lc_exp (term_to_exp t H).
+  intros t H H0.
+  induction H0 using lc_term_ind_4 with
+  (P0 := fun (a:gmargs) (H:lcA a) => forall (u:term), a = args u anil (cabs (var_b 0)) -> forall H : is_lambda u, lc_exp (term_to_exp u H))
+  (P1 := fun (l:alist) (H:lcL l) => forall (x:True), True)
+  (P2 := fun (c:cont) (H:lcC c) => forall (x:True), True); simpl; auto.
+  - constructor; intro.
+    change (lc_exp (open (term_to_exp t (il_abs_inv t H))
+                         (term_to_exp (L.var_f x) (il_var_f x)))).
+    unfold open_exp_wrt_exp.
+    assert (is_lambda (open_term_wrt_term_rec 0 (L.var_f x) t)).
+    apply open_preserves_il; inversion H; auto.
+    rewrite <- (term_to_exp_commutes_open _ _ _ _ 0 H1).
+    apply H0.
+  - inversion H; subst. constructor.
+    + trivial.
+    + apply IHlc_term0.
+      trivial.
+  - intros. inversion H1; subst.
+    apply IHlc_term.
+Qed.
 
 (* WIP: MP *)
 Module TEST.
@@ -325,93 +261,3 @@ Module TEST.
 
     Admitted.
 End TEST.
-
-Lemma term_to_exp_preserves_lc: forall t,
-    forall H, lcT t -> lc_exp (term_to_exp t H).
-  intros t H H0.
-  induction H0 using lc_term_ind_4 with
-  (P0 := fun (a:gmargs) (H:lcA a) => forall (u:term), a = args u anil (cabs (var_b 0)) -> forall H : is_lambda u, lc_exp (term_to_exp u H))
-  (P1 := fun (l:alist) (H:lcL l) => forall (x:True), True)
-  (P2 := fun (c:cont) (H:lcC c) => forall (x:True), True); simpl; auto.
-  - constructor; intro.
-    change (lc_exp (open (term_to_exp t (il_abs_inv t H))
-                         (term_to_exp (L.var_f x) (il_var_f x)))).
-    unfold open_exp_wrt_exp.
-    assert (is_lambda (open_term_wrt_term_rec 0 (L.var_f x) t)).
-    apply open_preserves_il; inversion H; auto.
-    rewrite <- (term_to_exp_commutes_open _ _ _ _ 0 H1).
-    apply H0.
-  - inversion H; subst. constructor.
-    + trivial.
-    + apply IHlc_term0.
-      trivial.
-  - intros. inversion H1; subst.
-    apply IHlc_term.
-Qed.
-
-
-Theorem term_to_exp_preserves_beta1: forall t u,
-forall (H1:is_lambda t) (H2:is_lambda u),
-beta1T t u -> beta (term_to_exp t H1) (term_to_exp u H2).
-Proof.
-  intros e1 e2 H1 H2 H. induction H. inversion H1; subst.
-  unfold open_term_wrt_term in *. simpl in *. inversion H6; subst.
-  rewrite (term_to_exp_commutes_open u t
-                                     (il_app_inv2 (abs t) u H1)
-                                     (il_abs_inv t (il_app_inv1 (abs t) u H1))).
-  apply beta_base.
-  - apply S.lc_abs. intro x.
-    change (S.lc_exp (open
-                        ((term_to_exp t) (il_abs_inv t (il_app_inv1 (abs t) u H1)))
-                        (term_to_exp (L.var_f x) (il_var_f x)))).
-    unfold open_exp_wrt_exp.
-    rewrite <- (term_to_exp_commutes_open _ _ _ _ 0 (open_preserves_il (L.var_f x) 
-                                                                    t (il_var_f x) H5 0)).
-    apply term_to_exp_preserves_lc. inversion H. apply H7.
-  - apply term_to_exp_preserves_lc. apply H0.
-Qed.
-
-(* Definition of full compatible closure of beta ---not in Stlc   *)
-
-Inductive ccBeta : exp -> exp -> Prop :=
- | ccBbase : forall (e1 e2:exp),
-     beta e1 e2 ->
-     ccBeta e1 e2
- | ccBapp1 : forall (e1 e2 e:exp),
-     ccBeta e1 e2 -> lc_exp e ->
-     ccBeta (S.app e1 e) (S.app e2 e)
- | ccBapp2 : forall (e1 e2 e:exp),
-     ccBeta e1 e2 -> lc_exp e ->
-     ccBeta (S.app e e1) (S.app e e2)
- | ccBabs : forall (e1 e2:exp) (L:vars),
-     (forall (x:var), x `notin` L ->
-                 ccBeta (open e1 (S.var_f x))  (open e2 (S.var_f x))) ->
-     ccBeta (S.abs e1) (S.abs e2).
-
-Hint Constructors ccBeta.
-
-Definition ccBeta1T := ccRTT beta1T.
-
-
-(* Simulation of one step beta reduction ---with compatible closure --by one step beta1 of LJm *)
-
-
-Theorem sim_by_ccbeta_term : forall e1 e2,
-    ccBeta e1 e2 -> ccBeta1T  (exp_to_terms e1) (exp_to_terms e2).
-Proof.
-  intros. induction H.
-  - intros. constructor. apply sim_by_beta_term. assumption.
-  - simpl. apply cc_app1.
-    + constructor;eauto.
-      * eapply lcT_from_lc_exp. assumption.
-      * constructor. intro. cbn. auto.
-    + fold ccBeta1T. assumption.
-  - simpl. apply cc_app2.
-    + eapply lcT_from_lc_exp. assumption.
-    + constructor; eauto. constructor. intro. cbn. auto.
-  - simpl. apply cc_abs with (L:=L). intros.
-    change (ccRTT beta1T (openT (exp_to_terms e1) (exp_to_terms (S.var_f x)))
-                  (openT (exp_to_terms e2) (exp_to_terms (S.var_f x)))).
-    repeat (rewrite <- commut_opens).  fold ccBeta1T.  specialize (H0 x). auto. 
-Qed.
-
