Lambda/Reduction.v
@@ -1,0 +1,73 @@
+Require Import ELambda.Definitions.
+
+Require Import Lambda.Syntax.
+Require Import LambdaJm.Syntax.
+Require Import LambdaJm.Reduction.
+
+Module S := ELambda.Definitions.
+Module L := LambdaJm.Syntax.
+
+Import S.ELambdaNotations.
+Import L.LambdaJmNotations.
+
+Lemma beta_preserves_il t1 t2 : is_lambda t1 -> betaT t1 t2 -> is_lambda t2.
+  intros.
+  induction H0.
+  - induction H0. inversion H. cbn.
+    inversion H5. apply open_preserves_il; trivial.
+  - induction H0. inversion H.
+Qed.
+
+
+Lemma sim_by_beta_term : forall e1 e2,
+    beta e1 e2 -> beta1T (exp_to_terms e1) (exp_to_terms e2).
+Proof.
+   intros. inversion H. simpl.  subst. rewrite  commut_opens. constructor.
+   - constructor. intro. inversion H0.
+     change ( lcT (openT (exp_to_terms e0) (exp_to_terms (S.var_f x)))).
+     rewrite <- commut_opens. specialize H3 with x. apply lcT_from_lc_exp. trivial.
+   - apply lcT_from_lc_exp. trivial.
+   - constructor. intro. cbn.  trivial.
+Qed.
+
+Theorem term_to_exp_preserves_beta1: forall t u,
+forall (H1:is_lambda t) (H2:is_lambda u),
+beta1T t u -> beta (term_to_exp t H1) (term_to_exp u H2).
+Proof.
+  intros e1 e2 H1 H2 H. induction H. inversion H1; subst.
+  unfold open_term_wrt_term in *. simpl in *. inversion H6; subst.
+  rewrite (term_to_exp_commutes_open u t
+                                     (il_app_inv2 (abs t) u H1)
+                                     (il_abs_inv t (il_app_inv1 (abs t) u H1))).
+  apply beta_base.
+  - apply S.lc_abs. intro x.
+    change (S.lc_exp (open
+                        ((term_to_exp t) (il_abs_inv t (il_app_inv1 (abs t) u H1)))
+                        (term_to_exp (L.var_f x) (il_var_f x)))).
+    unfold open_exp_wrt_exp.
+    rewrite <- (term_to_exp_commutes_open _ _ _ _ 0 (open_preserves_il (L.var_f x) 
+                                                                    t (il_var_f x) H5 0)).
+    apply term_to_exp_preserves_lc. inversion H. apply H7.
+  - apply term_to_exp_preserves_lc. apply H0.
+Qed.
+
+
+Theorem sim_by_ccbeta_term : forall (e1 e2:exp),
+    S.ccBeta e1 e2 -> ccBeta1T  (exp_to_terms e1) (exp_to_terms e2).
+Proof.
+  intros. induction H.
+  - intros. constructor. apply sim_by_beta_term. assumption.
+  - simpl. apply cc_app1.
+    + constructor;eauto.
+      * eapply lcT_from_lc_exp. assumption.
+      * constructor. intro. cbn. auto.
+    + fold ccBeta1T. assumption.
+  - simpl. apply cc_app2.
+    + eapply lcT_from_lc_exp. assumption.
+    + constructor; eauto. constructor. intro. cbn. auto.
+  - simpl. apply cc_abs with (L:=L). intros.
+    change (ccRTT beta1T (openT (exp_to_terms e1) (exp_to_terms (S.var_f x)))
+                  (openT (exp_to_terms e2) (exp_to_terms (S.var_f x)))).
+    repeat (rewrite <- commut_opens).  fold ccBeta1T.  specialize (H0 x). auto. 
+Qed.
+
