Lambda/Typing.v
@@ -1,0 +1,44 @@
+Require Import Lambda.Syntax.
+Require Import LambdaJm.Reduction.
+
+Module S := ELambda.Definitions.
+Module L := LambdaJm.Syntax.
+
+Import S.ELambdaNotations.
+Import L.LambdaJmNotations.
+
+
+(********
+ * Preservation of typing
+ ********)
+
+(* WIP: MP *)
+
+Lemma typing_implies_uniq G e A : typing G e A -> uniq G.
+  induction 1; trivial.
+Admitted.
+
+Theorem typing_preserved1 G e A : uniq G -> typing G e A -> typingT G (exp_to_terms e) A.
+  intros.
+  induction H0; simpl; auto.
+  - apply typingT_Right with (L:=L `union` dom G); intros.
+    simpl.
+    change (typingT ((x, T1) :: G) (openT (exp_to_terms e) (exp_to_terms (S.var_f x))) T2).
+    rewrite <- commut_opens.
+    apply H1; auto. 
+  - apply typingT_Cut with (A:=T1) (B:=T2).
+    + exact (IHtyping1 H).
+    + apply typingA_Leftm with (C:=T2).
+      * exact (IHtyping2 H).
+      * apply typingL_Ax. trivial.
+      * apply typingC_Select with (L:=dom G). intros.
+        apply typingT_Axiom.
+        -- auto.
+        -- auto.
+Qed.
+
+Theorem typing_preserved2 G t A : typingT G t A -> forall H : is_lambda t, typing G (term_to_exp2 t H) A.
+  intros.
+  admit.
+Admitted.
+
