LambdaJm/Lemmas.v
@@ -1,0 +1,80 @@
+
+(***********************************************************************)
+(** * Lemmas of LJm *)
+(***********************************************************************)
+
+(** This file containes lemmas for a locally-nameless
+    representation of the intuitionistic sequent calculus lambda-Jm .  *)
+
+
+Require Import Metalib.Metatheory.
+Require Import Stlc.Definitions.
+Require Import LJm.Definitions.
+
+Import LJmNotations.
+
+
+(*************************************************************************)
+(** ** Some proofs                                                       *)
+(*************************************************************************)
+
+
+(** The decidable var equality function returns a sum. If the two
+    vars are equal, the left branch of the sum is returned, carrying
+    a proof of the proposition that the vars are equal.  If they are
+    not equal, the right branch includes a proof of the disequality.
+
+    The demo below uses three new tactics:
+    - The tactic [simpl] reduces a Coq expression to its normal
+      form.
+    - The tactic [destruct (Y==Y)] considers the two possible
+      results of the equality test.
+*)
+
+
+Example demo_subst1:
+  [Y ~> var_f Z] (abs (app (var_b 0) (args (var_f Y) anil (cabs (var_b 0))))) =
+                  (abs (app (var_b 0) (args (var_f Z) anil (cabs (var_b 0))))).
+Proof.
+  simpl.
+  destruct (Y==Y).
+  - reflexivity.
+  - destruct n. auto.
+Qed. 
+
+
+(*************************************************************************)
+(** ** about testIN                                                      *)
+(*************************************************************************)
+
+(*************************************************************************)
+(** ** about append                                                      *)
+(*************************************************************************)
+
+(*************************************************************************)
+(** ** about typing                                                      *)
+(*************************************************************************)
+
+(*************************************************************************)
+(** ** Local closure *)
+(*************************************************************************)
+
+(** The local closure judgement classifies terms that have _no_ dangling
+   indices.
+
+   Step through this derivation to see why the term 
+   [((\x. Y (x,anil,(x)x)) (Y,anil,(x)x)]  is locally closed.
+*)
+
+(*************************************************************************)
+(** ** Properties about basic operations *)
+(*************************************************************************)
+
+(** The most important properties about open and lc concern their
+    relationship with the free variable and subst functions.
+
+    For example, one important property is shown below: that we can commute
+    free and bound variable substitution.
+ *)
+
+
