LambdaJm/Typing.v
@@ -1,0 +1,138 @@
+
+Require Import Metalib.Metatheory.
+Require Import LambdaJm.Syntax.
+
+Import LambdaJmNotations.
+
+
+(***********************************************************************)
+(** * Typing contexts *)
+(***********************************************************************)
+
+(** We represent typing contexts as association lists (lists of pairs of
+    keys and values) whose keys are [atom]s.
+*)
+
+Definition ctx : Set := list (var * typ).
+
+
+(***********************************************************************)
+(** * Typing relation for LJm *)
+(***********************************************************************)
+
+(** The typing rules handle four kinds of sequents, one per syntactic class. *)
+                                  
+(**  In order to ensure that the typing relation holds for only well-formed
+    environments, we check in the [typingT_var] case that the
+    environment is [uniq].  The structure of typing derivations
+    implicitly ensures that the relation holds only for locally closed
+    expressions.
+
+    Finally, note the use of cofinite quantification in
+    the [typingT_abs] case.
+*)
+
+Inductive typingT : ctx -> term -> typ -> Prop :=
+ | typingT_Axiom : forall (G:ctx) (x:var) (A:typ),
+     uniq G ->
+     binds x A G  ->
+     typingT G (var_f x) A
+ | typingT_Right : forall (L:vars) (G:ctx) (A:typ) (t:term) (B:typ),
+     (forall x , x `notin` L -> typingT ([(x,A)] ++ G) (t ^ x) B)  ->
+     typingT G (abs t) (typ_arrow A B)
+ | typingT_Cut : forall (G:ctx) (t:term) (a:gmargs) (A B C:typ),
+     typingT G t (typ_arrow A B) ->
+     typingA G (typ_arrow A B) a C ->
+     typingT G (app t a) C
+with typingA :  ctx -> typ -> gmargs -> typ -> Prop :=
+ | typingA_Leftm : forall (G:ctx) (u:term) (l:alist) (c:cont) (A B C D:typ),
+     typingT G u A ->
+     typingL G B l C ->
+     typingC G C c D ->
+     typingA G (typ_arrow A B) (args u l c) D
+with typingL :  ctx -> typ -> alist -> typ -> Prop :=
+ | typingL_Ax : forall (G:ctx) (C:typ),
+     uniq G ->
+     typingL G C anil C           
+ | typingL_Lft : forall (G:ctx) (u:term) (l:alist) (A B C:typ),
+     typingT G u A ->
+     typingL G B l C ->
+     typingL G (typ_arrow A B) (acons u l) C
+with typingC :  ctx -> typ -> cont -> typ -> Prop :=
+ | typingC_Select : forall (L:vars) (G:ctx) (C:typ) (v:term) (D:typ),
+     (forall x , x `notin` L -> typingT ([(x,C)] ++ G) (v ^ x) D)  ->
+     typingC G C (cabs v) D.
+
+
+Scheme typingT_ind_4 := Induction for typingT Sort Prop
+  with typingA_ind_4 := Induction for typingA Sort Prop
+  with typingL_ind_4 := Induction for typingL Sort Prop   
+  with typingC_ind_4 := Induction for typingC Sort Prop.
+
+
+Combined Scheme typing_mutind from
+         typingT_ind_4, typingA_ind_4, typingL_ind_4, typingC_ind_4.
+
+
+Hint Constructors typingT typingA typingL typingC.
+
+
+(***********************************************************************)
+(** * Results about typed reduction *)
+(***********************************************************************)
+
+Require Import LambdaJm.Reduction.
+
+
+Example ex1 : forall z A, typingT [(z,A)] (abs (var_b 0)) (typ_arrow A A).
+Proof.
+  intros z A. apply (typingT_Right {{z}}). intros x H. cbn. apply typingT_Axiom; fsetdec.
+Qed.
+
+Example ex2 : forall A, typingT nil (abs (var_b 0)) (typ_arrow A A).
+Proof.
+  intros A. apply (typingT_Right {}). intros x H. cbn. apply typingT_Axiom; fsetdec.
+Qed.
+
+Example ex3 : forall A B, typingT nil (abs (abs (var_b 1))) (typ_arrow A (typ_arrow B A)).
+Proof.
+  intros A B. apply (typingT_Right {}). intros x H. cbn. apply (typingT_Right {{x}}).
+  intros x0 H0. cbn.  apply typingT_Axiom; fsetdec.
+Qed.
+
+
+
+
+(* Contrary to proof of Lemma 3 in the paper, this proof is by induction in (typingL G A l B), 
+   rather than on induction on l (case viii) *)
+
+Lemma typing_app_alist_alist : (forall G A B C l',  typingL G B l' C ->
+    forall l, typingL G A l B -> typingL G A (app_alist_alist l l') C).
+Proof.
+  intros G A B C l' H l H0. induction H0.
+  - simpl. assumption.
+  - simpl. apply typingL_Lft.
+    + assumption.
+    + apply IHtypingL. assumption.
+Qed.
+
+
+
+(* Lemma 3 rules (ii) (iii) (iv)  *)
+Lemma typingApps : (forall G A B C1 C2 D a' a, typingA G (typ_arrow A B) a' (typ_arrow C1 C2) ->
+         typingA G (typ_arrow C1 C2) a D -> typingA G (typ_arrow A B) (app_args_args a' a) D) /\
+(forall G A B1 B2 C a c, typingC G A c (typ_arrow B1 B2) ->
+                    typingA G (typ_arrow B1 B2) a C -> typingC G A (app_cont_args c a) C)  /\
+(forall l:alist, True) /\
+(forall G A B C D x v a, typingT ([(x,D)] ++ G) v (typ_arrow A B) ->
+         typingA G (typ_arrow A B) a C -> typingT ([(x,D)] ++ G) (app_term_x_args v a) C).
+Proof.
+
+  (* apply (typing_mutind *)
+  (*        (fun G v C (H: typingT G v C) => (forall A B D x v a, typingT ([(x,D)] ++ G) v (typ_arrow A B) ->  typingA G (typ_arrow A B) a C -> typingT ([(x,D)] ++ G) (app_term_x_args v a) C)) *)
+  (*        (fun G A a' D (H: typingA G A a' D) => (forall C1 C2 a, typingA G A a' (typ_arrow C1 C2) -> typingA G (typ_arrow C1 C2) a D -> typingA G A (app_args_args a' a) D) ) *)
+  (*        (fun G A l D (H: typingL G A l D) => True ) *)
+  (*        (fun G A c C (H: typingC G A c C) => (forall B1 B2 a, typingC G A c (typ_arrow B1 B2) -> *)
+  (*           typingA G (typ_arrow B1 B2) a C -> typingC G A (app_cont_args c a) C)) ). *)
+
+Admitted.
